Constant propagate within expressions

theories/ValueOpts/ConstantPropagation.v
@@ -54,11 +54,34 @@ Definition exp_eval (E:onv (withTop val)) (e:exp) : aval :=
   | _ => Some Top
   end.
 
-Definition cp_choose_op E e :=
-  match op_eval E e with
-    | Some (wTA c) => Con c
-    | _ => e
-  end.
+Fixpoint cp_choose_op E e :=
+    match e with
+    | Con v => Con v
+    | Var x => match E x with
+              | Some (wTA v) => Con v
+              | _ => Var x
+              end
+    | UnOp o e =>
+      match cp_choose_op E e with
+      | Con v =>
+        match Val.unop_eval o v with
+        | Some v => Con v
+        | None => Con default_val
+        end
+      | e => UnOp o e
+      end
+    | BinOp o e1 e2 =>
+       match cp_choose_op E e1, cp_choose_op E e2 with
+       | Con v1, Con v2 =>
+         match Val.binop_eval o v1 v2 with
+         | Some v => Con v
+         | None => Con default_val
+         end
+       | Con v1, e => BinOp o (Con v1) e
+       | e, Con v2 => BinOp o e (Con v2)
+       | e1, e2 => BinOp o e1 e2
+       end
+    end.
 
 
 Fixpoint constantPropagate (AE:onv (withTop val)) s {struct s} : stmt :=
